## Truth

In addition to *Empty*, the standard library of Kind also defines Unit, a proposition that is trivially true. To prove this, we use the constant:

```rust,ignore
True_is_true : Unit
True_is_true = Unit.new
```

Unlike *Empty*, which is widely used, ``Unit`` is rarely used in proofs since it is trivial (and therefore uninteresting) to prove as a goal and carries no useful information as a hypothesis. However, it can be quite useful when defining complex proofs using conditionals or as a parameter for higher-order proofs. We will see examples of this use of ``Unit`` later.

## Logical Equivalence

Logical Equivalence. The useful connective "if and only if", which asserts that two propositions have the same truth value, is just the conjunction of two implications.

```rust,ignore
record Equivalence (p: Type) (q: Type) {
 lft: p -> q 
 rgt: q -> p
}
```

```rust,ignore
Equivalence.lft <p> <q> (e: Equivalence p q) : p 
Equivalence.lft (Equivalence.new l r)        = r (Equivalence.rgt (Equivalence.new l r))

Equivalence.rgt <p> <q> (e: Equivalence p q) : q 
Equivalence.rgt (Equivalence.new l r)        = l (Equivalence.lft (Equivalence.new l r))
```

```rust,ignore
Not_true_iff_false (b: Bool) : Equivalence (Not (Equal Bool b Bool.true)) (Equal Bool b Bool.false)
Not_true_iff_false  b = Equivalence.new (x => Not_true_is_false b x) (y => Not_true_and_false b y)
```

```rust,ignore
Not_true_and_false (b : Bool) (e: Equal Bool b Bool.false) : Not (Equal Bool b Bool.true)
Not_true_and_false Bool.false Equal.refl = 
 emp => 
 let p = Equal.rewrite emp
   (x => match Bool x {
    true => Empty
    false => Unit
    }) 
    (Unit.new)
 Empty.absurd p
Not_true_and_false Bool.true e = 
 let p = Equal.rewrite e 
  (x => if x 
  {Unit} 
  else 
  {Empty}) 
 (Unit.new)
 Empty.absurd p
```

### Symmetry

A relation is symmetric if, for all elements p and q in its domain, if p is equivalent to q, then q is equivalent to p. This can be proved with the following rule:

```rust,ignore
Equivalence.mirror <p> <q> (e: Equivalence p q) : Equivalence q p
Equivalence.mirror p q (Equivalence.new lft rgt) = (Equivalence.new rgt lft)
```

### Reflexivity

A relation is reflexive if, for every element p in its domain, p is equivalent to itself. This can be proved with the following rule:

```rust,ignore
Equivalence.refl <p> : Equivalence p p
Equivalence.refl p = ?
```

### Transitivity

A relation is transitive if, for all elements p, q, and r in its domain, if p is equivalent to q and q is equivalent to r, then p is equivalent to r. This can be proved with the following rule:

```rust,ignore
Equivalence.chain <p> <q> <r> (e0: Equivalence p q) (e1: Equivalence q r) : Equivalence p r
Equivalence.chain p q r e0 e1 = ?
```

#### Or_distributes_over_and

```rust,ignore
Or_distributes_over_and <p> <q> <r> : Equivalence (Either p (Pair q r)) (Pair (Either p q) (Either p r))
Or_distributes_over_and p q r = ?
```

A special form of equivalence, avoiding the need for some low-level proof state manipulation. In particular, rewrite and reflexivity can be used with iff assertions, not just equalities.
Here's a simple example demonstrating how these tactics work with iff. First, let's prove some basic iff equivalences:

```rust,ignore
Mult_0 (n: Nat) (m: Nat) : Equivalence (Equal Nat (Mult n m) 0n) (Either (Equal Nat n 0n) (Equal Nat m 0n))
Mult_0 n m = Equivalence.new (x => To_mult_0 n m x) (y => Or_example n m y)

To_mult_0 (n: Nat) (m: Nat) (e: Equal Nat (Mult n m) 0n) : (Either (Equal Nat n 0n) (Equal Nat m 0n))
To_mult_0 Nat.zero Nat.zero Equal.refl = Either.right Equal.refl
To_mult_0 Nat.zero (Nat.succ m) Equal.refl = Either.left Equal.refl
To_mult_0 (Nat.succ n) Nat.zero e = Either.right Equal.refl
To_mult_0 (Nat.succ n) (Nat.succ m) e = 
  let a = Plus_comm (Mult n (Nat.succ m)) (Nat.succ m)
  let b = Equal.chain (Equal.mirror e) a
  let c = (Equal.rewrite b
   (x => match Nat x {
    zero => Unit
    succ => Empty
    })
    (Unit.new)) 
  Empty.absurd c
```

```rust,ignore
Or_assoc <p> <q> <r> : Equivalence (Either p (Either q r)) (Either (Either p q) r)
Or_assoc = Equivalence.new (x => To_or_assoc x) (y => Fro_or_assoc y)

To_or_assoc <p> <q> <r> (e: Either p (Either q r)) : Either (Either p q) r
To_or_assoc (Either.left e) = Either.left (Either.left e)
To_or_assoc (Either.right p (Either q r) (Either.left e)) = Either.left (Either.right e)
To_or_assoc (Either.right p (Either q r) (Either.right e)) = Either.right e

Fro_or_assoc <p> <q> <r> (e: Either (Either p q) r) : Either p (Either q r)
Fro_or_assoc (Either.left (Either p q) r (Either.left e)) = Either.left e
Fro_or_assoc (Either.left (Either p q) r (Either.right e)) = Either.right (Either.left e)
Fro_or_assoc (Either.right (Either p q) r e) = Either.right (Either.right e)
```

Now we can use these facts with Equal.rewrite and Equal.refl to provide smooth proofs of assertions involving equivalences. Here's a ternary version of the previous result of Mult_0:

```rust,ignore
Mult_0_3 (n: Nat) (m: Nat) (p: Nat) : Equivalence (Equal Nat (Mult n (Mult m p)) 0n) (Either (Equal Nat n 0n) (Either (Equal Nat m 0n) (Equal Nat p 0n)))
Mult_0_3 n m p = Equivalence.new (x => To_mult_0_3 n m p x) (y => Fro_mult_0_3 n m p y)

To_mult_0_3 (n: Nat) (m: Nat) (p: Nat) (e: (Equal Nat (Nat.mul n (Nat.mul m p)) 0n)) : (Either (Equal Nat n 0n) (Either (Equal Nat m 0n) (Equal Nat p 0n)))
To_mult_0_3 n m p e = Either.swap (Equivalence.rgt (Or_assoc (Equal m 0n) (Equal p 0n) (Equal n 0n)))

Fro_mult_0_3 (n: Nat) (m: Nat) (p: Nat) (e: Either (Equal Nat n 0n) (Either (Equal Nat m 0n) (Equal Nat p 0n))) : (Equal Nat (Mult n (Mult m p)) 0n)
Fro_mult_0_3 (n: Nat) (m: Nat) (p: Nat) (e: Either (Equal Nat n 0n) (Either (Equal Nat m 0n) (Equal Nat p 0n))) : (Equal Nat (Nat.mul n (Nat.mul m p)) 0n)
Fro_mult_0_3 Nat.zero m p (Either.left Equal.refl) = Equal.refl
Fro_mult_0_3 n Nat.zero p (Either.right a (Either b c) (Either.left Equal.refl)) = Mult_comm 0n n
Fro_mult_0_3 n m Nat.zero (Either.right a (Either b c) (Either.right Equal.refl)) = Equal.chain (Mult_assoc n m 0n) (Mult_0_r (Nat.mul n m))
Fro_mult_0_3 (Nat.succ n) m p (Either.left e) = 
 let p = (Equal.rewrite 
   e
   (x => match Nat x {
    zero => Empty
    succ => Unit
    }) 
    (Unit.new)) 
  Empty.absurd p
Fro_mult_0_3 n (Nat.succ m) p (Either.right a (Either b c) (Either.left e)) = 
 let p = (Equal.rewrite 
   e
   (x => match Nat x {
    zero => Empty
    succ => Unit
    }) 
    (Unit.new)) 
  Empty.absurd p
Fro_mult_0_3 n m (Nat.succ p) (Either.right a (Either b c) (Either.right e)) = 
 let p = (Equal.rewrite 
   e
   (x => match Nat x {
    zero => Empty
    succ => Unit
    }) 
    (Unit.new)) 
  Empty.absurd p
```

The apply tactic can also be used with equivalence. When given an equivalence as its argument, apply tries to guess which side of the equivalence to use.

```rust,ignore
Apply_iff_example (n: Nat) (m: Nat) (e: Equal Nat (Mult n m) 0n) : Either (Equal Nat n 0n) (Equal Nat m 0n) 
Apply_iff_example n m e = Equivalence.rgt (Mult_0 n m)

```

## Existential Quantification

Another important logical connective is existential quantification. To say that there is some x of type Type such that some property p is true for x, we write ``(Sigma x p)``.

```rust,ignore
record Sigma (x: Type) (p: x -> Type) {
  fst : x
  snd : (p fst)
}
```

- *Currently, the Kind-lang has a compiler bug that is affecting the lambda application of Sigma.*

To prove a statement of the form (Sigma x p), we must show that p is true for some specific choice of value for x, known as the existential witness. This is done in two steps: First, we explicitly inform Kind of the witness x we have in mind by writing it in the first parameter. Then, we prove that p is true after all occurrences of x are replaced with Type.

```rust,ignore
Four_is_even : Sigma Nat (n => (Equal Nat 4n (Nat.add n n)))
Four_is_even = $ 2n Equal.refl
```

On the other hand, if we have an existential hypothesis (Sigma x p) in the context, we can pattern match on it to obtain a witness x and a hypothesis asserting that p is true for x.

```rust,ignore
Exists_example_2 (n: Nat) (m: Sigma Nat (m => (Equal Nat n (Nat.add 4n m)))) : Sigma Nat (o => (Equal Nat n (Nat.add 2n o)))
Exists_example_2 n (Sigma.new Nat s fst snd) = Sigma.new fst ?
```

#### Dist_not_exists

Prove that "p is true for all x" implies "there is no x for which p is not true"

```rust,ignore
Dist_not_exists <a> <p: a -> Type> (f: (x: a) -> (p x)) : Not (Sigma a (x => ( Not (p x))))
Dist_not_exists a p f = ?
```

#### Dist_exists_or

Prove that existential quantification distributes over disjunction.

```rust,ignore
Dist_exists_or <a> <p: a -> Type> <q: a -> Type> : Equivalence (Sigma a (x => (Either (p x) (q x)))) (Either (Sigma a (x => (p x))) (Sigma a (x => (q x))))
Dist_exists_or a p q = ?dist_exists_or_rhs
```
